Parsing/Tree.v
@@ -4,7 +4,8 @@ Require Import
         List 
         Ascii
         String
-        Syntax.Regex.
+        Syntax.Regex
+        Utils.Functions.ListUtils.
 
 Import ListNotations.
 
@@ -16,12 +17,38 @@ Inductive tree : Set :=
 | TCat  : tree -> tree -> tree
 | TStar : list tree -> tree.
 
+
 Section TREE_IND.
   Variable P : tree -> Prop.
   Variable Q : list tree -> Prop.
 
   Hypothesis
-    (H : 
+    (HTEps: P TEps)
+    (HTChr : forall a, P (TChr a))
+    (HTLeft : forall t, P t -> P (TLeft t))
+    (HTRight : forall t, P t -> P (TRight t))
+    (HTCat : forall t, P t -> forall t', P t' -> P (TCat t t'))
+    (H : forall (ts : list tree), Q ts -> P (TStar ts))
+    (H0 : Q (@nil tree))
+    (H1 : forall (t : tree),
+        P t ->
+        forall (ts : list tree), Q ts -> Q (t :: ts)).
+  
+  Fixpoint tree_ind_full (t : tree) : P t :=
+    match t as x return P x with
+    | TEps       => HTEps
+    | TChr a     => HTChr a
+    | TLeft t    => HTLeft (tree_ind_full t)
+    | TRight t   => HTRight (tree_ind_full t)
+    | TCat t t'  => HTCat (tree_ind_full t) (tree_ind_full t') 
+    | TStar ts   => 
+      H ((fix l_ind (ts' : list tree) : Q ts' :=
+            match ts' as x return Q x with
+            | [] => H0
+            | t' :: ts'' => H1 (tree_ind_full t') (l_ind ts'')
+            end) ts)
+    end.
+End TREE_IND.
 
 Inductive is_tree_of : tree -> regex -> Prop :=
 | ITEps : is_tree_of TEps #1
@@ -31,8 +58,10 @@ Inductive is_tree_of : tree -> regex -> Prop :=
 | ITCat : forall tl tr l r, is_tree_of tl l ->
                        is_tree_of tr r ->
                        is_tree_of (TCat tl tr) (l @ r)
-| ITStar : forall e ts, Forall (fun t => is_tree_of t e) ts ->
-                   is_tree_of (TStar ts)  (e ^*).
+| ITStarEnd : forall e, is_tree_of (TStar []) (Star e)
+| ITStarRec : forall e ts t, is_tree_of t e ->
+                        is_tree_of (TStar ts) (Star e) ->
+                        is_tree_of (TStar (t :: ts)) (Star e).
 
 Hint Constructors is_tree_of.
 
@@ -43,14 +72,17 @@ Fixpoint flat (t : tree) : string :=
   | TLeft t => flat t
   | TRight t => flat t
   | TCat t t' => flat t ++ flat t'
-  | TStar ts => fold_right (fun t ac => flat t ++ ac) "" ts
+  | TStar ts => fold_right (fun t ac => flat t ++ ac) "" ts 
   end.
+
+Lemma str_append_rewind
+  : forall s s' a, String a (s ++ s') = (String a s) ++ s'.
+Proof.
+  induction s ; crush.
+Qed.
 
 Lemma flat_correct : forall t e, is_tree_of t e -> (flat t) <<- e.
 Proof.
-  induction 1 ; crush.
-  +
-    eapply InCat ; eauto.
-  +
-    
+  intros t e H ; induction H ; crush ; eauto.
+  destruct (flat t) eqn : Ha ; eauto.
 Qed.
